lib/Types.v
@@ -1,12 +1,12 @@
 Require Import List.
 
-Class Serializer A := {
+Class Serializer A :=
+  {
     serialize: A -> (list bool);
     deserialize: list bool -> option (A * list bool);
-    Serialize_reversible: forall x: A,
-                            deserialize (serialize x) = Some (x, nil) }.
-
-Print serialize.
+    Serialize_reversible: forall (x: A) (bin: list bool),
+                            deserialize ((serialize x) ++ bin) = Some (x, bin)
+  }.
 
 Definition bool_serialize (a: bool) : list bool :=
   a :: nil.
@@ -17,8 +17,8 @@ Definition bool_deserialize (bin : list bool) : option (bool * list bool) :=
     | h :: t => Some (h, t)
   end.
 
-Lemma bool_serialize_reversible: forall x: bool,
-                                   bool_deserialize (bool_serialize x) = Some (x, nil).
+Lemma bool_serialize_reversible: forall (x: bool) (bin: list bool),
+                                   bool_deserialize ((bool_serialize x) ++ bin) = Some (x, bin).
   intros; simpl.
   reflexivity.
 Qed.
@@ -26,6 +26,8 @@ Qed.
 Instance Bool_Serializer: Serializer bool :=
   {
     serialize := bool_serialize;
-    deserialize := bool_deserialize;
-    Serialize_reversible := bool_serialize_reversible
+    deserialize := bool_deserialize
   }.
+intros; simpl.
+reflexivity.
+Qed.
